custom masks to replace (buggy?) FStar.UInt*.eq_mask, etc.

src/QUIC.Secret.Int.fst
@@ -1,4 +1,5 @@
 module QUIC.Secret.Int
+module Aux = QUIC.Secret.Int.Aux
 
 let usub
   #t #sec x y
@@ -26,211 +27,15 @@ let lognot'
 = U.nth_lemma #(bits t) (U.lognot (v x)) (v x `U.logxor` v (ones t l));
   x `logxor` ones t l
 
-let logand_one_bit
-  #t #sec x y
-= x `mul` y
+let logand_one_bit = Aux.logand_one_bit
 
-let logor_one_bit_8
-  (sec: secrecy_level)
-  (x: int_t U8 sec { v x == 0 \/ v x == 1 })
-  (y: int_t U8 sec { v y == 0 \/ v y == 1 })
-: Lemma
-  (v (x `logor` y) == (if v x = 1 || v y = 1 then 1 else 0))
-= logor_spec x y;
-  allow_inversion secrecy_level;
-  assert (U8.logor 0uy 0uy == 0uy);
-  assert (U8.logor 0uy 1uy == 1uy);
-  assert (U8.logor 1uy 0uy == 1uy);
-  assert (U8.logor 1uy 1uy == 1uy)
+let logor_one_bit = Aux.logor_one_bit
 
-let logor_one_bit_16
-  (sec: secrecy_level)
-  (x: int_t U16 sec { v x == 0 \/ v x == 1 })
-  (y: int_t U16 sec { v y == 0 \/ v y == 1 })
-: Lemma
-  (v (x `logor` y) == (if v x = 1 || v y = 1 then 1 else 0))
-= logor_spec x y;
-  allow_inversion secrecy_level;
-  assert (U16.logor 0us 0us == 0us);
-  assert (U16.logor 0us 1us == 1us);
-  assert (U16.logor 1us 0us == 1us);
-  assert (U16.logor 1us 1us == 1us)
+let logxor_one_bit = Aux.logxor_one_bit
 
-let logor_one_bit_32
-  (sec: secrecy_level)
-  (x: int_t U32 sec { v x == 0 \/ v x == 1 })
-  (y: int_t U32 sec { v y == 0 \/ v y == 1 })
-: Lemma
-  (v (x `logor` y) == (if v x = 1 || v y = 1 then 1 else 0))
-= logor_spec x y;
-  allow_inversion secrecy_level;
-  assert (U32.logor 0ul 0ul == 0ul);
-  assert (U32.logor 0ul 1ul == 1ul);
-  assert (U32.logor 1ul 0ul == 1ul);
-  assert (U32.logor 1ul 1ul == 1ul)
+let secret_bool = Aux.secret_bool
 
-let logor_one_bit_64
-  (sec: secrecy_level)
-  (x: int_t U64 sec { v x == 0 \/ v x == 1 })
-  (y: int_t U64 sec { v y == 0 \/ v y == 1 })
-: Lemma
-  (v (x `logor` y) == (if v x = 1 || v y = 1 then 1 else 0))
-= logor_spec x y;
-  allow_inversion secrecy_level;
-  assert (U64.logor 0uL 0uL == 0uL);
-  assert (U64.logor 0uL 1uL == 1uL);
-  assert (U64.logor 1uL 0uL == 1uL);
-  assert (U64.logor 1uL 1uL == 1uL)
-
-let logor_one_bit'
-  (#t: inttype { supported_type t })
-  (#sec: secrecy_level)
-  (x: int_t t sec { v x == 0 \/ v x == 1 })
-  (y: int_t t sec { v y == 0 \/ v y == 1 })
-: Lemma
-  (v (x `logor` y) == (if v x = 1 || v y = 1 then 1 else 0))
-= match t with
-  | U8 -> logor_one_bit_8 sec x y
-  | U16 -> logor_one_bit_16 sec x y
-  | U32 -> logor_one_bit_32 sec x y
-  | U64 -> logor_one_bit_64 sec x y
-
-let logor_one_bit
-  #t #sec x y
-= logor_one_bit' x y;
-  x `logor` y
-
-let logxor_one_bit_8
-  (sec: secrecy_level)
-  (x: int_t U8 sec { v x == 0 \/ v x == 1 })
-  (y: int_t U8 sec { v y == 0 \/ v y == 1 })
-: Lemma
-  (v (x `logxor` y) == (if v x = v y then 0 else 1))
-= logxor_spec x y;
-  allow_inversion secrecy_level;
-  assert (U8.logxor 0uy 0uy == 0uy);
-  assert (U8.logxor 0uy 1uy == 1uy);
-  assert (U8.logxor 1uy 0uy == 1uy);
-  assert (U8.logxor 1uy 1uy == 0uy)
-
-let logxor_one_bit_16
-  (sec: secrecy_level)
-  (x: int_t U16 sec { v x == 0 \/ v x == 1 })
-  (y: int_t U16 sec { v y == 0 \/ v y == 1 })
-: Lemma
-  (v (x `logxor` y) == (if v x = v y then 0 else 1))
-= logxor_spec x y;
-  allow_inversion secrecy_level;
-  assert (U16.logxor 0us 0us == 0us);
-  assert (U16.logxor 0us 1us == 1us);
-  assert (U16.logxor 1us 0us == 1us);
-  assert (U16.logxor 1us 1us == 0us)
-
-let logxor_one_bit_32
-  (sec: secrecy_level)
-  (x: int_t U32 sec { v x == 0 \/ v x == 1 })
-  (y: int_t U32 sec { v y == 0 \/ v y == 1 })
-: Lemma
-  (v (x `logxor` y) == (if v x = v y then 0 else 1))
-= logxor_spec x y;
-  allow_inversion secrecy_level;
-  assert (U32.logxor 0ul 0ul == 0ul);
-  assert (U32.logxor 0ul 1ul == 1ul);
-  assert (U32.logxor 1ul 0ul == 1ul);
-  assert (U32.logxor 1ul 1ul == 0ul)
-
-let logxor_one_bit_64
-  (sec: secrecy_level)
-  (x: int_t U64 sec { v x == 0 \/ v x == 1 })
-  (y: int_t U64 sec { v y == 0 \/ v y == 1 })
-: Lemma
-  (v (x `logxor` y) == (if v x = v y then 0 else 1))
-= logxor_spec x y;
-  allow_inversion secrecy_level;
-  assert (U64.logxor 0uL 0uL == 0uL);
-  assert (U64.logxor 0uL 1uL == 1uL);
-  assert (U64.logxor 1uL 0uL == 1uL);
-  assert (U64.logxor 1uL 1uL == 0uL)
-
-let logxor_one_bit'
-  (#t: inttype { supported_type t })
-  (#sec: secrecy_level)
-  (x: int_t t sec { v x == 0 \/ v x == 1 })
-  (y: int_t t sec { v y == 0 \/ v y == 1 })
-: Lemma
-  (v (x `logxor` y) == (if v x = v y then 0 else 1))
-= match t with
-  | U8 -> logxor_one_bit_8 sec x y
-  | U16 -> logxor_one_bit_16 sec x y
-  | U32 -> logxor_one_bit_32 sec x y
-  | U64 -> logxor_one_bit_64 sec x y
-
-let logxor_one_bit
-  #t #sec x y
-= logxor_one_bit' x y;
-  x `logxor` y
-
-let secret_bool
-  #t #sec x
-= cast t sec (if x then 1uy else 0uy)
-
-let lognot_one_bit
-  #t #sec x
-= x `logxor_one_bit` secret_bool true
-
-(* Conversion between HACL*'s 00/FF style and our 0/1 style *)
-
-[@"opaque_to_smt"]
-noextract
-inline_for_extraction
-let ff00_to_10
-  (#t: inttype { supported_type t })
-  (#sec: secrecy_level)
-  (x: int_t t sec { v x == 0 \/ v x == U.ones (bits t) })
-: Tot (y: int_t t sec { v y == (if v x = 0 then 0 else 1) })
-= U.logand_lemma_1 #(bits t) 1;
-  U.logand_lemma_2 #(bits t) 1;
-  mk_int 1 `logand` x
-
-(* Comparisons *)
-
-noextract
-[@"opaque_to_smt"]
-inline_for_extraction
-let secrets_are_equal
-  (#t: inttype { supported_type t })
-  (size: nat)
-  (x: int_t t SEC { v x < pow2 size })
-  (y: int_t t SEC { v y < pow2 size })
-: Tot (z: int_t t SEC {
-    v z == (if v x = v y then 1 else 0)
-  })
-= eq_mask_lemma #t x y;
-  ff00_to_10 (eq_mask #t x y)
-
-noextract
-[@"opaque_to_smt"]
-inline_for_extraction
-let secret_is_lt
-  (#t: inttype { supported_type t })
-  (size: nat { size <= bits t })
-  (x: int_t t SEC { v x < pow2 (size) })
-  (y: int_t t SEC { v y < pow2 (size) })
-: Tot (z: int_t t SEC { v z == (if v x < v y then 1 else 0) })
-  (decreases (size))
-= lt_mask_lemma #t x y;
-  ff00_to_10 (lt_mask #t x y)
-
-noextract
-[@"opaque_to_smt"]
-inline_for_extraction
-let secret_is_le
-  (#t: inttype { supported_type t })
-  (size: nat { size <= bits t })
-  (x: int_t t SEC { v x < pow2 (size) })
-  (y: int_t t SEC { v y < pow2 (size) })
-: Tot (z: int_t t SEC { v z == (if v x <= v y then 1 else 0) })
-= secret_is_lt size x y `logor_one_bit` secrets_are_equal size x y
+let lognot_one_bit = Aux.lognot_one_bit
 
 #push-options "--z3rlimit 64"
 
@@ -253,38 +58,43 @@ let set_bitfield
 
 (* Instances *)
 
+
 let secrets_are_equal_32_2
-  x y
-= (secrets_are_equal 2 x y)
+  (x: uint32 { v x < pow2 2 })
+  (y: uint32 { v y < pow2 2 })
+: Tot (z: uint32 {
+    v z == (if v x = v y then 1 else 0)
+  })
+= norm [delta_attr [(`%Aux.must_inline)]; iota; zeta; primops] (Aux.secrets_are_equal 2 x y)
 
 let secret_is_le_64
-  x y
-= (secret_is_le 64 x y)
+  (x: uint64)
+  (y: uint64)
+: Tot (z: uint64 { v z == (if v x <= v y then 1 else 0) })
+= norm [delta_attr [(`%Aux.must_inline)]; iota; zeta; primops] (Aux.secret_is_le 64 x y)
 
 let secret_is_lt_64
-  x y
-= (secret_is_lt 64 x y)
+  (x: uint64)
+  (y: uint64)
+: Tot (z: uint64 { v z == (if v x < v y then 1 else 0) })
+= norm [delta_attr [(`%Aux.must_inline)]; iota; zeta; primops] (Aux.secret_is_lt 64 x y)
 
 let secrets_are_equal_64_2
-  x y
-= (secrets_are_equal 2 x y)
+  (x: uint64 { v x < pow2 2 })
+  (y: uint64 { v y < pow2 2 })
+: Tot (z: uint64 {
+    v z == (if v x = v y then 1 else 0)
+  })
+= norm [delta_attr [(`%Aux.must_inline)]; iota; zeta; primops] (Aux.secrets_are_equal 2 x y)
 
 let secrets_are_equal_62
-  x y
-= (secrets_are_equal 62 x y)
+  (x: uint64 { v x < pow2 62 })
+  (y: uint64 { v y < pow2 62 })
+: Tot (z: uint64 {
+    v z == (if v x = v y then 1 else 0)
+  })
+= norm [delta_attr [(`%Aux.must_inline)]; iota; zeta; primops] (Aux.secrets_are_equal 62 x y)
 
-#push-options "--z3rlimit 16"
+let min64 = Aux.min64
 
-let min
-  #t x y
-=
-  let cond = secret_is_le (bits t) x y in
-  (cond `mul` x) `add` (lognot_one_bit cond `mul` y)
-
-let max
-  #t x y
-=
-  let cond = secret_is_le (bits t) y x in
-  (cond `mul` x) `add` (lognot_one_bit cond `mul` y)
-
-#pop-options
+let max64 = Aux.max64
